coq/JsSyntaxAux.v
@@ -9,10 +9,11 @@ Implicit Type l : object_loc.
 
 (** Builds an object with all optional fields to None *)
 
-Definition object_create vproto sclass bextens P :=
+Definition object_create vproto sclass bextens builtinget P :=
   {| object_proto_ := vproto;
      object_class_ := sclass;
      object_extensible_ := bextens;
+     object_get_ := builtinget;
      object_properties_ := P;
      object_prim_value_ := None;
      object_construct_ := None;
@@ -30,31 +31,31 @@ Definition object_create vproto sclass bextens P :=
 
 Definition object_with_properties O properties :=
   match O with
-  | object_intro x1 x2 x3 x4 x5 x6 x7 x8 x9 x10 x11 x12 x13 x14 x15 =>
-    object_intro x1 x2 x3 properties x5 x6 x7 x8 x9 x10 x11 x12 x13 x14 x15
+  | object_intro x1 x2 x3 x4 x5 x6 x7 x8 x9 x10 x11 x12 x13 x14 x15 x16 =>
+    object_intro x1 x2 x3 x4 properties x6 x7 x8 x9 x10 x11 x12 x13 x14 x15 x16
   end.
 
 (** Modifies the primitive value field of an object *)
 
 Definition object_with_primitive_value O v :=
   match O with
-  | object_intro x1 x2 x3 x4 x5 x6 x7 x8 x9 x10 x11 x12 x13 x14 x15 =>
-    object_intro x1 x2 x3 x4 (Some v) x6 x7 x8 x9 x10 x11 x12 x13 x14 x15
+  | object_intro x1 x2 x3 x4 x5 x6 x7 x8 x9 x10 x11 x12 x13 x14 x15 x16 =>
+    object_intro x1 x2 x3 x4 x5 (Some v) x7 x8 x9 x10 x11 x12 x13 x14 x15 x16
   end.
 
 (** Modifies the construct, call and has_instance fields of an object *)
 Definition object_with_invokation O constr call has_instance :=
   match O with
-  | object_intro x1 x2 x3 x4 x5 x6 x7 x8 x9 x10 x11 x12 x13 x14 x15 =>
-    object_intro x1 x2 x3 x4 x5 constr call has_instance x9 x10 x11 x12 x13 x14 x15
+  | object_intro x1 x2 x3 x4 x5 x6 x7 x8 x9 x10 x11 x12 x13 x14 x15 x16 =>
+    object_intro x1 x2 x3 x4 x5 x6 constr call has_instance x10 x11 x12 x13 x14 x15 x16
   end.
 
 (** Modifies the other parameters of an object *)
 
 Definition object_with_details O scope params code target boundthis boundargs paramsmap :=
   match O with
-  | object_intro x1 x2 x3 x4 x5 x6 x7 x8 x9 x10 x11 x12 x13 x14 x15 =>
-    object_intro x1 x2 x3 x4 x5 x6 x7 x8 scope params code target boundthis boundargs paramsmap
+  | object_intro x1 x2 x3 x4 x5 x6 x7 x8 x9 x10 x11 x12 x13 x14 x15 x16 =>
+    object_intro x1 x2 x3 x4 x5 x6 x7 x8 x9 scope params code target boundthis boundargs paramsmap
   end.
 
 
@@ -282,7 +283,7 @@ Qed.
 
 Global Instance object_inhab : Inhab object.
 Proof.
-  apply (prove_Inhab (object_create arbitrary arbitrary arbitrary arbitrary)).
+  apply (prove_Inhab (object_create arbitrary arbitrary arbitrary arbitrary arbitrary)).
 Qed.
 
 
